\documentclass{../templates/topic}

\title{State Space to Transfer Function}
\author{Daniel "lilatomic" Goldman}

\begin{document}
\maketitle

\begin{section}{Definition}
	The TF can be derived simply with the application of the formula
	\begin{equation}
		G(s)=\frac{Y}{U}=(C\cdot INV[s\vec{1}-A]\cdot B+D)
	\end{equation}
\end{section}

\begin{section}{Derivation}
	
	With
	\begin{align}
		\dot{X}&=AX+BU\\
		Y&=CX+DU
	\end{align}
	The $\laplace$ gives
	\begin{align}
		\laplace{X}(s)&=sX(s)=AX+BU(s)\\
		\laplace{Y}(s)&=\ Y(s)=CX(s)+DU(s)
	\end{align}
	Rearanging gives
	\begin{align}
		(s\vec{1}-A)X(s)&=BU(s)\\
		X(s)&=(s\vec{1}-A)BU(s)\\
	\end{align}
	And substituting $X(s)$ from above
	\begin{equation}
		Y(s)=(C\cdot INV[s\vec{1}-A]\cdot B+D)U(s)
	\end{equation}
\end{section}

\end{document}